src/Analysis/Instances/Product/Ctx/Int_Ctx_Call_String_Sound.thy
@@ -36,7 +36,7 @@ definition ics_eqs ::
        \<Rightarrow> pname \<Rightarrow> com
        \<Rightarrow> (pp \<times> call_string, call_string_gk, (int_dom exec_dg_st lifted, int_dom exec_dg_st lifted) dg_state) eqsT" where
   "ics_eqs k mode gs is_bot_pred Pi ps mnm main =
-     side_cfg_T_eff_keyed_seed_dg_buffered intra_predecessor_list (\<lambda>_. Call_String_Context.Global)
+     side_cfg_T_eff_keyed_seed_dg_buffered intra_predecessor_addr_list (\<lambda>_. Call_String_Context.Global)
        (cs_route k)
        (routed_cmb_g_contribution (ictx_spec mode is_bot_pred gs) Call_String_Context.Global Call_String_Context.Seed)
        (routed_extra_g Call_String_Context.Seed Call_String_Context.Global)
@@ -123,7 +123,7 @@ lemma ics_pp_st:
 
 theorem ics_pp_abs:
   "part_post_solution
-     (side_cfg_T_eff_keyed_seed_dg intra_predecessor_list (\<lambda>_. Call_String_Context.Global) (cs_route k)
+     (side_cfg_T_eff_keyed_seed_dg intra_predecessor_addr_list (\<lambda>_. Call_String_Context.Global) (cs_route k)
         (routed_cmb_g (ictx_abs_spec mode gs) Call_String_Context.Global Call_String_Context.Seed)
         (routed_extra_g Call_String_Context.Seed Call_String_Context.Global)
         (compile_prog Pi ps mnm main) (ictx_abs_spec mode gs)
@@ -136,7 +136,7 @@ theorem ics_pp_abs:
      (fst (ics_sol k mode gs is_bot_pred Pi ps mnm main))"
 proof -
   have pp_buf: "part_post_solution
-       (side_cfg_T_eff_keyed_seed_dg_buffered intra_predecessor_list
+       (side_cfg_T_eff_keyed_seed_dg_buffered intra_predecessor_addr_list
           (\<lambda>_. Call_String_Context.Global) (cs_route k)
           (routed_cmb_g_contribution (ictx_spec mode is_bot_pred gs)
              Call_String_Context.Global Call_String_Context.Seed)
