src/Analysis/Instances/Sign/Ctx/Sign_Ctx_Call_String_Sound.thy
@@ -35,7 +35,7 @@ definition scs_eqs ::
     "nat \<Rightarrow> (vname \<Rightarrow> bool) \<Rightarrow> (sign exec_dg_st \<Rightarrow> bool) \<Rightarrow> proc_table \<Rightarrow> pname list \<Rightarrow> pname \<Rightarrow> com
        \<Rightarrow> (pp \<times> call_string, call_string_gk, (sign exec_dg_st lifted, sign exec_dg_st lifted) dg_state) eqsT" where
   "scs_eqs k gs is_bot_pred Pi ps mnm main =
-     side_cfg_T_eff_keyed_seed_dg_buffered intra_predecessor_list (\<lambda>_. Call_String_Context.Global)
+     side_cfg_T_eff_keyed_seed_dg_buffered intra_predecessor_addr_list (\<lambda>_. Call_String_Context.Global)
        (cs_route k)
        (routed_cmb_g_contribution (sctx_spec gs is_bot_pred) Call_String_Context.Global Call_String_Context.Seed)
        (routed_extra_g Call_String_Context.Seed Call_String_Context.Global)
@@ -120,7 +120,7 @@ lemma scs_pp_st:
 
 theorem scs_pp_abs:
   "part_post_solution
-     (side_cfg_T_eff_keyed_seed_dg intra_predecessor_list (\<lambda>_. Call_String_Context.Global) (cs_route k)
+     (side_cfg_T_eff_keyed_seed_dg intra_predecessor_addr_list (\<lambda>_. Call_String_Context.Global) (cs_route k)
         (routed_cmb_g (sctx_abs_spec gs) Call_String_Context.Global Call_String_Context.Seed)
         (routed_extra_g Call_String_Context.Seed Call_String_Context.Global)
         (compile_prog Pi ps mnm main) (sctx_abs_spec gs)
@@ -133,7 +133,7 @@ theorem scs_pp_abs:
      (fst (scs_sol k gs is_bot_pred Pi ps mnm main))"
 proof -
   have pp_buf: "part_post_solution
-       (side_cfg_T_eff_keyed_seed_dg_buffered intra_predecessor_list
+       (side_cfg_T_eff_keyed_seed_dg_buffered intra_predecessor_addr_list
           (\<lambda>_. Call_String_Context.Global) (cs_route k)
           (routed_cmb_g_contribution (sctx_spec gs is_bot_pred)
              Call_String_Context.Global Call_String_Context.Seed)
