src/Analysis/Instances/Sign/Ctx/Sign_Ctx_Entry_State_Sound.thy
@@ -68,7 +68,7 @@ definition sctx_entry_eqs ::
     "(vname \<Rightarrow> bool) \<Rightarrow> (sign exec_dg_st \<Rightarrow> bool) \<Rightarrow> proc_table \<Rightarrow> pname list \<Rightarrow> pname \<Rightarrow> com
        \<Rightarrow> (pp \<times> sign list, gk, (sign exec_dg_st lifted, sign exec_dg_st lifted) dg_state) eqsT" where
   "sctx_entry_eqs gs is_bot_pred Pi ps mnm main =
-     side_cfg_T_eff_keyed_seed_dg_buffered intra_predecessor_list (\<lambda>_. Global)
+     side_cfg_T_eff_keyed_seed_dg_buffered intra_predecessor_addr_list (\<lambda>_. Global)
        (sctx_entry_route_gen gs is_bot_pred)
        (routed_cmb_g_contribution (sctx_spec gs is_bot_pred) Global Seed)
        (routed_extra_g Seed Global)
@@ -175,7 +175,7 @@ lemma sctx_entry_pp_st:
 
 theorem sctx_entry_pp_abs:
   "part_post_solution
-     (side_cfg_T_eff_keyed_seed_dg intra_predecessor_list (\<lambda>_. Global)
+     (side_cfg_T_eff_keyed_seed_dg intra_predecessor_addr_list (\<lambda>_. Global)
         (formals_route_lifted_gen (sctx_abs_spec gs))
         (routed_cmb_g (sctx_abs_spec gs) Global Seed)
         (routed_extra_g Seed Global)
@@ -189,7 +189,7 @@ theorem sctx_entry_pp_abs:
      (fst (sctx_entry_sol gs is_bot_pred Pi ps mnm main))"
 proof -
   have pp_buf: "part_post_solution
-       (side_cfg_T_eff_keyed_seed_dg_buffered intra_predecessor_list (\<lambda>_. Global)
+       (side_cfg_T_eff_keyed_seed_dg_buffered intra_predecessor_addr_list (\<lambda>_. Global)
           (sctx_entry_route_gen gs is_bot_pred)
           (routed_cmb_g_contribution (sctx_spec gs is_bot_pred) Global Seed)
           (routed_extra_g Seed Global)
@@ -296,7 +296,7 @@ proof unfold_locales
   show "finite (intra (compile_prog Pi ps mnm main))" by (rule sctx_entry_fin)
 next
   show "part_post_solution
-          (side_cfg_T_eff_keyed_seed_dg intra_predecessor_list (\<lambda>_. Global)
+          (side_cfg_T_eff_keyed_seed_dg intra_predecessor_addr_list (\<lambda>_. Global)
              (formals_route_lifted_gen (sctx_abs_spec gs))
              (routed_cmb_g (sctx_abs_spec gs) Global Seed)
              (routed_extra_g Seed Global)
